src/Generators.v
@@ -1,19 +1,18 @@
 Set Warnings "-extraction-opaque-accessed,-extraction".
 Set Warnings "-notation-overridden,-parsing".
 
-Require Import ZArith List.
+From Coq Require Import String List ZArith Lia.
 Require Import mathcomp.ssreflect.ssreflect.
-From mathcomp Require Import ssrfun ssrbool ssrnat seq.
-Require Import Numbers.BinNums.
-Require Import Classes.RelationClasses.
+From mathcomp Require Import ssrfun ssrbool ssrnat eqtype seq.
 
-From ExtLib.Structures Require Export
+(*From ExtLib.Structures Require Export
      Monads.
 From ExtLib.Structures Require Import
      Functor Applicative.
-Import MonadNotation.
+*)
+(* Import MonadNotation.
 Open Scope monad_scope.
-
+*)
 From QuickChick Require Import
      RandomQC RoseTrees Sets Tactics Producer.
 
@@ -121,6 +120,14 @@ Definition sample1 (A : Type) (g : G A) : A :=
         m 10 rnd
     end.
 
+Lemma runFmap (A B : Type) (f : A -> B) (g : G A) seed size :
+    run (fmap f g) size seed = f (run g size (fst (randomSplit seed))).
+Proof. simpl.
+       destruct (randomSplit seed).
+       simpl.
+       auto.
+Qed.
+
 (* Generator specific - shrinking support. *)
 Definition promote {A : Type} (m : Rose (G A)) : G (Rose A) :=
     MkGen (fun n r => fmapRose (fun g => run g n r) m).
@@ -156,7 +163,7 @@ Lemma semPromote A (m : Rose (G A)) :
 Proof. by rewrite /codom2 curry_codom2l. Qed.
 
 Lemma semPromoteSize (A : Type) (m : Rose (G A)) n :
-    semGenSize (promote m) n <-->
+    semProdSize (promote m) n <-->
                codom (fun seed => fmapRose (fun g => run g n seed) m).
 Proof. by []. Qed.
 
@@ -172,7 +179,7 @@ Definition choose {A : Type} `{ChoosableFromInterval A} (range : A * A) : G A :=
 
 Lemma semChooseSize A `{ChoosableFromInterval A} (a1 a2 : A) :
     RandomQC.leq a1 a2 ->
-    forall size, semGenSize (choose (a1,a2)) size <-->
+    forall size, semProdSize (choose (a1,a2)) size <-->
                        [set a | RandomQC.leq a1 a && RandomQC.leq a a2].
 Proof. by move=> /= le_a1a2 m n; rewrite (randomRCorrect n a1 a2). Qed.
   
@@ -207,7 +214,6 @@ Qed.
           `{@Unsized _ _ ProducerGen (f tt)} : Unsized (thunkGen f).
   Proof.
     intros s1 s2.
-    Set Printing All.
     do 2 rewrite semThunkGenSize.
     apply unsized.
   Qed.
@@ -247,7 +253,7 @@ Fixpoint pick {A : Type} (def : G A) (xs : list (nat * G A)) n : nat * G A :=
 (* This should use urns! *)
 Fixpoint pickDrop {A : Type} (xs : list (nat * G (option A))) n : nat * G (option A) * list (nat * G (option A)) :=
   match xs with
-    | nil => (0, returnGen None, nil)
+    | nil => (0, ret None, nil)
     | (k, x) :: xs =>
       if (n < k) then  (k, x, xs)
       else let '(k', x', xs') := pickDrop xs (n - k)
@@ -270,12 +276,12 @@ Definition frequency {A}:=
 
 Fixpoint backtrackFuel {A : Type} (fuel : nat) (tot : nat) (gs : list (nat * G (option A))) : G (option A) :=
   match fuel with 
-    | O => returnGen None
+    | O => ret None
     | S fuel' => bindGen (choose (0, tot-1)) (fun n => 
                  let '(k, g, gs') := pickDrop gs n in
                  bindGen g (fun ma =>
                  match ma with 
-                   | Some a => returnGen (Some a)
+                   | Some a => ret (Some a)
                    | None => backtrackFuel fuel' (tot - k) gs'
                  end ))
   end.
@@ -328,7 +334,408 @@ Definition suchThatMaybeOpt {A : Type} (g : G (option A))
 Definition retrySized {A : Type} (g : G (option A)) : G (option A) :=
   sized (fun n => retry n g).
 
+(* begin semReturn *)
+Lemma semReturnGen {A} (x : A) : semProd (ret x) <--> [set x].
+(* end semReturn *)
+Proof.
+  rewrite /semProd /semProdSize /= /semGenSize /=
+  bigcup_const ?codom_const //.
+  exact: randomSeed_inhabited.
+    by do 2! constructor.
+Qed.
+  
+Lemma semReturnSizeGen A (x : A) (s : nat) :
+  semProdSize (ret x) s <--> [set x].
+Proof.
+  rewrite /semProdSize /= /semGenSize.
+  rewrite codom_const; [ reflexivity | apply randomSeed_inhabited ].
+Qed.
+
+Lemma randomSplit_codom : codom randomSplit <--> setT.
+Proof.
+by apply/subset_eqP; split=> // [[s1 s2]] _; apply: randomSplitAssumption.
+Qed.
 
 
+Lemma semBindSizeGen A B (g : G A) (f : A -> G B) (s : nat) :
+    semGenSize (bindGen g f) s <-->
+    \bigcup_(a in semGenSize g s) semGenSize (f a) s.
+Proof.
+    rewrite /semGenSize /bindGen /= bigcup_codom -curry_codom2l.
+    by rewrite -[codom (prod_curry _)]imsetT -randomSplit_codom -codom_comp.
+Qed.
+
+Lemma semChooseGen A `{RandomQC.ChoosableFromInterval A} (a1 a2 : A) :
+    RandomQC.leq a1 a2 ->
+    (semProd (choose (a1,a2)) <--> [set a | RandomQC.leq a1 a && RandomQC.leq a a2]).
+Proof.
+  move=> /= le_a1a2. rewrite <- (unsized_alt_def 1).
+  move => m /=. rewrite (randomRCorrect m a1 a2) //.
+Qed.
 
   
+Lemma semChooseSizeGen A `{ChoosableFromInterval A} (a1 a2 : A) :
+    RandomQC.leq a1 a2 ->
+    forall size, semGenSize (choose (a1,a2)) size <-->
+                       [set a | RandomQC.leq a1 a && RandomQC.leq a a2].
+Proof. by move=> /= le_a1a2 m n; rewrite (randomRCorrect n a1 a2). Qed.
+
+Lemma  semChooseSizeEmptyGen :
+    forall A `{RandomQC.ChoosableFromInterval A} (a1 a2 : A),
+      ~ (RandomQC.leq a1 a2) ->
+      forall size, (semProdSize (choose (a1,a2)) size <-->
+                                set0).
+Admitted.  
+
+
+Lemma semSizedGen A (f : nat -> G A) :
+    semProd (sized f) <--> \bigcup_n semGenSize (f n) n.
+Proof. by []. Qed.
+
+Lemma semSizedSizeGen A (f:nat->G A)s : semGenSize (sized f) s <--> semGenSize (f s) s.
+Proof. by []. Qed.
+
+Lemma semResizeGen A n (g : G A) : semProd (resize n g) <--> semGenSize g n .
+Proof.
+   by case: g => g; rewrite /semProd /semProdSize /= /semGenSize /= bigcup_const.
+Qed.
+
+Lemma semResizeSizeGen A (s n : nat) (g : G A) :
+    semGenSize (resize n g) s <--> semGenSize g n.
+Proof. by case: g => g; rewrite /semGenSize. Qed.
+
+Global Instance ProducerSemanticsGen :
+  @ProducerSemantics G ProducerGen :=
+  {
+  semReturn     := @semReturnGen; 
+  semReturnSize := @semReturnSizeGen;
+  semBindSize   := @semBindSizeGen;
+  semChoose     := @semChooseGen;
+  semChooseSize := @semChooseSizeGen;
+  semChooseSizeEmpty := @semChooseSizeEmptyGen;
+  semSized      := @semSizedGen;
+  semSizedSize  := @semSizedSizeGen;
+  semResize     := @semResizeGen;
+  semResizeSize := @semResizeSizeGen
+  }.
+
+Module QcDefaultNotation.
+
+Declare Scope qc_scope.
+
+Notation " 'elems' [ x ] " := (elems_ x (cons x nil)) : qc_scope.
+Notation " 'elems' [ x ; y ] " := (elems_ x (cons x (cons y nil))) : qc_scope.
+Notation " 'elems' [ x ; y ; .. ; z ] " :=
+  (elems_ x (cons x (cons y .. (cons z nil) ..))) : qc_scope.
+Notation " 'elems' ( x ;; l ) " :=
+  (elems_ x (cons x l)) (at level 1, no associativity) : qc_scope.
+
+Notation " 'oneOf' [ x ] " := (oneOf_ x (cons x nil)) : qc_scope.
+Notation " 'oneOf' [ x ; y ] " := (oneOf_ x (cons x (cons y nil))) : qc_scope.
+Notation " 'oneOf' [ x ; y ; .. ; z ] " :=
+  (oneOf_ x (cons x (cons y .. (cons z nil) ..))) : qc_scope.
+Notation " 'oneOf' ( x ;; l ) " :=
+  (oneOf_ x (cons x l))  (at level 1, no associativity) : qc_scope.
+
+Notation " 'freq' [ x ] " := (freq_ x nil) : qc_scope.
+Notation " 'freq' [ ( n , x ) ; y ] " :=
+  (freq_ x (cons (n, x) (cons y nil))) : qc_scope.
+Notation " 'freq' [ ( n , x ) ; y ; .. ; z ] " :=
+  (freq_ x (cons (n, x) (cons y .. (cons z nil) ..))) : qc_scope.
+Notation " 'freq' ( ( n , x ) ;; l ) " :=
+  (freq_ x (cons (n, x) l)) (at level 1, no associativity) : qc_scope.
+
+End QcDefaultNotation.
+
+Section FrequencyProof.
+(* A rather long frequency proof, probably we can do better *)
+
+Lemma not_lt : forall n m, (false = (n < m)) -> (m <= n).
+Proof.
+  move => n m. by elim: n m=> [| n IHn]; case.
+Qed.
+
+Lemma sum_fstE A x (a : A) l:
+  sum_fst ((x, a) :: l) = x + sum_fst l.
+Proof.
+rewrite /sum_fst /=.
+elim: l 0 x => [n x|[n1 x1] l IHl p q] /=; first by rewrite addnC.
+by rewrite -IHl; congr foldl; rewrite addnAC.
+Qed.
+
+Lemma sum_fst_eq0P {A} (l : list (nat * A)) :
+  sum_fst l = 0 <->
+  [seq x <- l | x.1 != 0] = [::].  
+Proof.
+by elim: l => [|[[|n] x] l IHl] //=; split=> //; rewrite sum_fstE.
+Qed.
+
+Lemma pick_def :
+  forall {A} (l: list (nat * G A)) n def,
+    sum_fst l <= n ->
+    pick def l n = (0, def).
+Proof.
+  move=> A l n def Hleq.
+  elim : l n Hleq => //=. case=> //= i p l IHl n Hleq.
+  rewrite sum_fstE in Hleq.
+  remember (n < i). case: b Heqb => Heqb; symmetry in Heqb.
+  - have : (i + sum_fst l) < i by eapply (leq_ltn_trans); eassumption.
+    rewrite -ltn_subRL. by have -> : forall i, (i - i) = 0 by elim.
+  - apply IHl. rewrite -(leq_add2r i) subnK.
+      by rewrite addnC. by apply/not_lt.
+Qed.
+
+Lemma pick_exists :
+  forall {A} (l: list (nat * G A)) n def,
+    n <  sum_fst l <->
+    exists x, List.In x l /\ pick def l n = x /\ fst x <> 0.
+Proof.
+  move => A l n def. split.
+  - move => Hlt.
+    elim : l n Hlt => //. case => i p xs IHxs n Hlt.
+    rewrite sum_fstE in Hlt.
+    move/(_ (n-i)) : IHxs => IHxs. simpl.
+    remember (n < i). case: b Heqb => [Heqb | /not_lt Heqb].
+    + exists (i, p). split => //=. by left.  split => //=.
+      move => contra; subst. by rewrite ltn0 in Heqb.
+    + rewrite -(ltn_add2r i) [X in _  < X]addnC subnK // in IHxs.
+      move/(_ Hlt) : IHxs => [x [H1 [H2 H3]]].
+      by exists x; split; [right | split].
+  - move => [x [HIn [Hpick Hneq]]].
+    remember (n < sum_fst l).
+    case: b  Heqb => //= /not_lt/pick_def H.
+    rewrite H in Hpick. rewrite -Hpick //= in Hneq.
+Qed.
+
+Lemma pick_In :
+  forall {A} (l: list (nat * G A)) x def,
+    List.In x l /\ fst x <> 0 ->
+    exists n, pick def l n = x.
+Proof.
+  move => A l x def [HIn Hfst].
+  elim : l HIn => //=. case => //= i g xs IHxs [H1 | H2]; subst.
+  + exists 0. simpl in *.
+    have H : 0 < i by  elim : i Hfst IHxs => //=.
+    rewrite H.
+      by split => //=.
+  + move/(_ H2) : IHxs => [n Hpick].
+    exists (n + i). rewrite -[X in _ < X]add0n ltn_add2r ltn0.
+      by rewrite  -[X in _ - X]add0n subnDr subn0.
+Qed.
+
+Lemma pick_imset A (def : G A) l :
+  pick def l @: [set m | m < sum_fst l] <--> [seq x <- l | x.1 != 0]. 
+Proof.
+elim: l => [|[n x] l IHl] /=.
+  rewrite /sum_fst /=.
+  have->: (fun m => m < 0) <--> set0 by [].
+  by rewrite imset0.
+case: n => /= [|n].
+  rewrite -IHl => t; split=> [[y []]|].
+    by rewrite sum_fstE add0n subn0 => lt_y <-; exists y.
+  by case=> y [lt_y <-]; exists y; split=> //; rewrite subn0.
+move=> t; split=> /= [[p [lt_p]]|].
+  case: ifP => [_ <-|lt_pn ?]; first by left.
+    right; rewrite -(IHl t); exists (p - n.+1); split=> //.
+  rewrite sum_fstE in lt_p.
+  by rewrite -(ltn_add2r n.+1) subnK 1?addnC // leqNgt lt_pn.
+case=> [<-|]; first by exists 0; split => //; rewrite sum_fstE.
+rewrite -(IHl t); case=> p [lt_p <-]; exists (n.+1 + p); split.
+  by rewrite sum_fstE ltn_add2l.
+by rewrite ltnNge leq_addr addKn.
+Qed.
+
+Lemma pickDrop_def :
+  forall {A} (l: list (nat * G (option A))) n,
+    sum_fst l <= n ->
+    pickDrop l n = (0, ret None, l).
+Proof.
+  move=> A l n Hleq.
+  elim : l n Hleq => //=. case=> //= i p l IHl n Hleq.
+  rewrite sum_fstE in Hleq.
+  remember (n < i). case: b Heqb => Heqb; symmetry in Heqb.
+  - have : (i + sum_fst l) < i by eapply (leq_ltn_trans); eassumption.
+    rewrite -ltn_subRL. by have -> : forall i, (i - i) = 0 by elim.
+  - rewrite IHl; auto. rewrite -(leq_add2r i) subnK.
+      by rewrite addnC. by apply/not_lt.
+Qed.
+
+(* Probably needs something about l' and l. *)
+(* ZP : added a few things *)
+Lemma pickDrop_exists :
+  forall {A} (l: list (nat * G (option A))) n,
+    n <  sum_fst l <->
+    exists k g l',
+      List.In (k,g) l /\ pickDrop l n = (k,g,l') /\ k <> 0 /\
+      l <--> [set (k, g)] :|: l' /\
+      length l' + 1 = length l /\
+      sum_fst l' + k = sum_fst l.
+Proof.
+  move => A l n. split.
+  - move => Hlt.
+    elim : l n Hlt => //. case => i p xs IHxs n Hlt.
+    rewrite sum_fstE in Hlt.
+    move/(_ (n-i)) : IHxs => IHxs. simpl.
+    remember (n < i). case: b Heqb => [Heqb | /not_lt Heqb].
+    + exists i. exists p. exists xs. split => //=. by left.  split => //=.
+      split. move => contra; subst. by rewrite ltn0 in Heqb.
+      split. by rewrite cons_set_eq.
+      split. by ssromega.
+      rewrite sum_fstE. by ssromega.
+    + rewrite -(ltn_add2r i) [X in _  < X]addnC subnK // in IHxs.
+      move/(_ Hlt) : IHxs => [k [g [gs [H1 [H2 [H3 [H4 [H5 H6]]]]]]]].
+      exists k. exists g. exists ((i,p)::gs).
+      split; [right | split; [| split; [| split; [| split]]]];
+      try (simpl; eauto; by rewrite H2).
+      rewrite !cons_set_eq H4.
+      rewrite setU_assoc (setU_comm [set (i, p)]) -setU_assoc.
+      reflexivity.
+      simpl. by ssromega.
+      simpl. rewrite !sum_fstE. by ssromega.
+  - move => [k [g [gs [HIn [Hpick [Hneq _]]]]]].
+    remember (n < sum_fst l).
+    case: b  Heqb => //= /not_lt/pickDrop_def H.
+    rewrite H in Hpick. 
+    inversion Hpick; subst; eauto.
+Qed.
+
+Lemma pickDrop_In :
+  forall {A} (l: list (nat * G (option A))) k x,
+    List.In (k,x) l /\ k <> 0 ->
+    exists n l', pickDrop l n = (k,x,l').
+Proof.
+  move => A l k x [HIn Hfst].
+  elim : l HIn => //=. case => //= i g xs IHxs [H1 | H2]; subst.
+  + exists 0.  exists xs. simpl in *.
+    inversion H1; subst; clear H1.
+    have H : 0 < k by  elim : k Hfst IHxs => //=.
+    rewrite H.
+      by split => //=.
+  + move/(_ H2) : IHxs => [n [l' Hpick]].
+    exists (n + i). exists ((i,g)::l'). 
+    rewrite -[X in _ < X]add0n ltn_add2r ltn0.
+    rewrite  -[X in _ - X]add0n subnDr subn0.
+    by rewrite Hpick.
+Qed.
+
+Lemma pickDrop_In_strong :
+  forall {A} (l: list (nat * G (option A))) k x,
+    List.In (k,x) l /\ k <> 0 ->
+    exists n l',
+      pickDrop l n = (k,x,l') /\
+      n < sum_fst l /\
+      length l = length l' + 1.
+Proof.
+  move => A l k x [HIn Hfst].
+  elim : l HIn => //=. case => //= i g xs IHxs [H1 | H2]; subst.
+  + exists 0.  exists xs. simpl in *.
+    inversion H1; subst; clear H1.
+    have H : 0 < k by  elim : k Hfst IHxs => //=.
+    rewrite H. split ; [| split ]; simpl; auto.
+    rewrite sum_fstE. now ssromega.
+    now ssromega.
+  + move/(_ H2) : IHxs => [n [l' [Hpick [Hlt Hlen]]]].
+    exists (n + i). exists ((i,g)::l'). 
+    rewrite -[X in _ < X]add0n ltn_add2r ltn0.
+    rewrite  -[X in _ - X]add0n subnDr subn0.
+    rewrite Hpick. simpl.
+    split ; [| split ]; simpl; auto.
+    rewrite sum_fstE. now ssromega.
+    now ssromega.
+Qed.
+
+(* begin semFrequencySize *)
+Lemma semFrequencySize {A}
+      (l : list (nat * G A)) (def : G A) (size: nat) :
+  semProdSize (freq_ def l) size <-->
+    let l' := [seq x <- l | x.1 != 0] in
+    if l' is nil then semProdSize def size else
+      \bigcup_(x in l') semProdSize x.2 size.
+(* end semFrequencySize *)
+Proof.
+rewrite semBindSize semChooseSize //=.
+case lsupp: {1}[seq x <- l | x.1 != 0] => [|[n g] gs].
+move/sum_fst_eq0P: lsupp => suml; rewrite suml.
+  rewrite (@eq_bigcupl _ _ _ [set 0]) ?bigcup_set1 ?pick_def // ?leqn0 ?suml //.
+  by move=> n; split; rewrite leqn0; [move/eqP|] => ->.
+symmetry; apply: reindex_bigcup.
+have pos_suml: 0 < sum_fst l.
+  have [] := sum_fst_eq0P l.
+  by rewrite lsupp; case: (sum_fst l) => // /(_ erefl).
+have->: (fun a : nat => a <= sum_fst l - 1) <--> [set m | m < sum_fst l].
+  by move=> m /=; rewrite -ltnS subn1 prednK.
+exact: pick_imset.
+Qed.
+
+(* begin semFrequency *)
+Lemma semFrequency {A} (l : list (nat * G A)) (def : G A) :
+  semProd (freq_ def l) <-->
+    let l' := [seq x <- l | x.1 != 0] in
+    if l' is nil then semProd def else
+      \bigcup_(x in l') semProd x.2.
+(* end semFrequency *)
+Proof.
+by case lsupp: {1}[seq x <- l | x.1 != 0] => [|[n g] gs] /=;
+rewrite 1?bigcupC; apply: eq_bigcupr => sz;
+have := (semFrequencySize l def sz); rewrite lsupp.
+Qed.
+
+Lemma frequencySizeMonotonic {A} (g0 : G A) lg :
+  SizeMonotonic g0 ->
+  List.Forall (fun p => SizeMonotonic (snd p)) lg ->
+  SizeMonotonic (freq_ g0 lg).
+Proof.
+  intros H1.  unfold freq_.
+  intros Hall. eapply bindMonotonicStrong.
+  - eauto with typeclass_instances.
+  - apply unsizedMonotonic.
+    apply chooseUnsized.
+  - intros x Heq. eapply semChoose in Heq; eauto.  
+  move : Heq => /andP [Hep1 Heq2]. 
+  destruct (sum_fst lg) eqn:Heq.
+  + rewrite pick_def. eassumption.
+    subst. ssromega.
+  + edestruct (pick_exists lg x g0) as [[[n' g] [Hin [Hp Hg]]] H2].
+    rewrite Heq. unfold leq, RandomQC.super, ChooseNat, OrdNat in Hep1, Heq2.
+    ssromega.
+    eapply List.Forall_forall in Hall; [ | ].
+    eassumption.
+    subst. rewrite Hp. eassumption.
+Qed.
+
+Instance frequencySizeMonotonic_alt :
+  forall {A : Type} (g0 : G A) (lg : seq (nat * G A)),
+    SizeMonotonic g0 ->
+    lg \subset [set x | SizeMonotonic x.2 ] ->
+    SizeMonotonic (freq_ g0 lg).
+Proof.
+  intros A g ls Hm Hin.
+  eapply frequencySizeMonotonic. eassumption.
+  induction ls. now constructor.
+  constructor. eapply Hin.
+  constructor. reflexivity.
+  eapply IHls.  eapply subset_trans; eauto.
+  constructor 2. eassumption.
+Qed.
+
+End FrequencyProof.  
+
+Definition bindGenOpt {A B}
+           (g : G (option A)) (f : A -> G (option B)) : G (option B) :=
+  bindGen g (fun ma =>
+    match ma with
+    | None => returnGen None
+    | Some a => f a
+    end).
+  
+(* Backwards compatibility. *)
+Definition elements := @elems_ G ProducerGen.
+Definition liftGen := @liftM G (@super _ ProducerGen).
+Definition liftGen2 := @liftM2 G (@super _ ProducerGen).
+Definition liftGen3 := @liftM3 G (@super _ ProducerGen).
+Definition liftGen4 := @liftProd4 _ ProducerGen.
+Definition liftGen5 := @liftProd5 _ ProducerGen.
+Definition sequenceGen := @sequenceProd G ProducerGen.
+Definition oneof := @oneOf_ G ProducerGen.
+Definition frequency := @freq_.
+Definition semGen := @semProd G ProducerGen.
